disk-betree/ImplDealloc.i.dfy
@@ -18,30 +18,6 @@ module ImplDealloc {
 
   import opened NativeTypes
 
-  method Deallocable(s: ImplVariables, ref: BT.G.Reference) returns (result: bool)
-  requires s.W()
-  requires s.ready ==> s.ephemeralIndirectionTable.Inv()
-  ensures result == ImplModelDealloc.deallocable(s.I(), ref)
-  {
-    if ref == BT.G.Root() {
-      return false;
-    }
-    assert ref != BT.G.Root();
-    if !s.ready {
-      return false;
-    }
-    assert s.ready;
-    var lbaGraph := s.ephemeralIndirectionTable.Get(ref);
-    if !lbaGraph.Some? {
-      return false;
-    }
-    assert ref in IM.IIndirectionTable(IIndirectionTable(s.ephemeralIndirectionTable)).graph;
-    var table := s.ephemeralIndirectionTable.ToMap();
-    var graph := map k | k in table :: table[k].1;
-    assert graph == IM.IIndirectionTable(IIndirectionTable(s.ephemeralIndirectionTable)).graph;
-    result := forall r | r in graph :: ref !in graph[r];
-  }
-
   method Dealloc(k: ImplConstants, s: ImplVariables, io: DiskIOHandler, ref: BT.G.Reference)
   requires Inv(k, s)
   requires io.initialized()
@@ -56,13 +32,10 @@ module ImplDealloc {
     ImplModelDealloc.reveal_Dealloc();
 
     if s.frozenIndirectionTable != null {
-      var lbaGraph := s.frozenIndirectionTable.Get(ref);
-      if lbaGraph.Some? {
-        var (lba, _) := lbaGraph.value;
-        if lba.None? {
-          print "giving up; dealloc can't dealloc because frozen isn't written\n";
-          return;
-        }
+      var b := s.frozenIndirectionTable.HasEmptyLoc(ref);
+      if b {
+        print "giving up; dealloc can't run because frozen isn't written";
+        return;
       }
     }
 
@@ -73,17 +46,14 @@ module ImplDealloc {
 
     ImplModelCache.lemmaIndirectionTableLocIndexValid(Ic(k), s.I(), ref);
 
-    var oldEntry := s.ephemeralIndirectionTable.RemoveAndGet(ref);
+    var oldLoc := s.ephemeralIndirectionTable.RemoveRef(ref);
 
     s.lru.Remove(ref);
     s.cache.Remove(ref);
 
-    if oldEntry.Some? && oldEntry.value.0.Some? {
-      s.blockAllocator.MarkFreeEphemeral(oldEntry.value.0.value.addr / BlockSizeUint64());
+    if oldLoc.Some? {
+      s.blockAllocator.MarkFreeEphemeral(oldLoc.value.addr / BlockSizeUint64());
     }
-
-    assume s.ephemeralIndirectionTable.Contents
-        == MapRemove(old(s.ephemeralIndirectionTable.Contents), {ref});
 
     ghost var s1 := s.I();
     ghost var s2 := ImplModelDealloc.Dealloc(Ic(k), old(s.I()), old(IIO(io)), ref).0;
@@ -105,26 +75,6 @@ module ImplDealloc {
   ensures ref == ImplModelDealloc.FindDeallocable(s.I())
   {
     ImplModelDealloc.reveal_FindDeallocable();
-
-    // TODO once we have an lba freelist, rewrite this to avoid extracting a `map` from `s.ephemeralIndirectionTable`
-    var ephemeralTable := s.ephemeralIndirectionTable.ToMap();
-    var ephemeralRefs := SetToSeq(ephemeralTable.Keys);
-
-    assume |ephemeralRefs| < 0x1_0000_0000_0000_0000;
-
-    var i: uint64 := 0;
-    while i < |ephemeralRefs| as uint64
-    invariant 0 <= i as int <= |ephemeralRefs|
-    invariant ImplModelDealloc.FindDeallocableIterate(s.I(), ephemeralRefs, i)
-           == ImplModelDealloc.FindDeallocable(s.I())
-    {
-      var ref := ephemeralRefs[i];
-      var isDeallocable := Deallocable(s, ref);
-      if isDeallocable {
-        return Some(ref);
-      }
-      i := i + 1;
-    }
-    return None;
+    ref := s.ephemeralIndirectionTable.FindDeallocable();
   }
 }
