disk-betree/IndirectionTableModel.i.dfy
@@ -1,0 +1,571 @@
+include "../lib/Maps.s.dfy"
+include "../lib/sequences.s.dfy"
+include "../lib/Option.s.dfy"
+include "../lib/NativeTypes.s.dfy"
+include "../lib/LRU.i.dfy"
+include "../lib/MutableMapModel.i.dfy"
+include "PivotBetreeSpec.i.dfy"
+include "AsyncSectorDiskModel.i.dfy"
+include "BlockCacheSystem.i.dfy"
+include "../lib/Marshalling/GenericMarshalling.i.dfy"
+include "../lib/Bitmap.i.dfy"
+
+module IndirectionTableModel {
+  import opened Maps
+  import opened Sets
+  import opened Options
+  import opened Sequences
+  import opened NativeTypes
+  import ReferenceType`Internal
+  import BT = PivotBetreeSpec`Internal
+  import BC = BetreeGraphBlockCache
+  import LruModel
+  import MutableMapModel
+  import LBAType
+  import opened GenericMarshalling
+  import Bitmap
+  import opened Bounds
+
+  datatype Entry = Entry(loc: Option<BC.Location>, succs: seq<BT.G.Reference>)
+  type HashMap = MutableMapModel.LinearHashMap<Entry>
+
+  // TODO move bitmap in here?
+  datatype IndirectionTable = IndirectionTable(
+    t: HashMap,
+    locs: map<BT.G.Reference, BC.Location>,
+    graph: map<BT.G.Reference, seq<BT.G.Reference>>
+  )
+
+    // This contains reference with the empty predecessor set.
+    // We use a LRU queue not because we care about the LRU,
+    // but just because it happens to be a queue data structure lying around.
+    //garbageQueue: LruModel.LruQueue,
+    //refcounts: map<BT.G.Reference, uint64>)
+
+  function Locs(t: HashMap) : map<BT.G.Reference, BC.Location>
+  {
+    map ref | ref in t.contents && t.contents[ref].loc.Some? :: t.contents[ref].loc.value
+  }
+
+  function Graph(t: HashMap) : map<BT.G.Reference, seq<BT.G.Reference>>
+  {
+    map ref | ref in t.contents :: t.contents[ref].succs
+  }
+
+  /*datatype PredecessorEdge = PredecessorEdge(src: BT.G.Reference, idx: int)
+
+  function PredecessorSet(graph: map<BT.G.Reference, seq<BT.G.Reference>>, dest: BT.G.Reference) : set<PredecessorEdge>
+  {
+    set src, idx | src in graph && 0 <= idx < graph[src] :: PredecessorEdge(src, idx)
+  }
+
+  function GraphRefcounts(graph: map<BT.G.Reference, seq<BT.G.Reference>>) : map<BT.G.Reference, uint64>
+  {
+    map ref | ref in graph :: |PredecessorSet(graph, ref)|
+  }
+
+  predicate Refcount0(self: IndirectionTable, ref: BT.G.Reference)
+  {
+    && ref in refcounts
+    && refcounts[ref] == 0
+  }
+  */
+
+  protected predicate Inv(self: IndirectionTable)
+  ensures Inv(self) ==> (forall ref | ref in self.locs :: ref in self.graph)
+  {
+    //&& (forall ref | ref in LruModel.I(self.garbageQueue) :: Refcount0(self, ref))
+    //&& (forall ref | Refcount0(self, ref) :: ref in LruModel.I(self.garbageQueue))
+    //&& self.refcounts == GraphRefcounts(self.graph)
+    && MutableMapModel.Inv(self.t)
+    && self.locs == Locs(self.t)
+    && self.graph == Graph(self.t)
+  }
+
+  function IHashMap(m: HashMap) : BC.IndirectionTable
+  {
+    BC.IndirectionTable(Locs(m), Graph(m))
+  }
+
+  function I(self: IndirectionTable) : BC.IndirectionTable
+  {
+    BC.IndirectionTable(self.locs, self.graph)
+  }
+
+  function FromHashMap(m: HashMap) : IndirectionTable
+  requires MutableMapModel.Inv(m)
+  ensures Inv(FromHashMap(m))
+  {
+    IndirectionTable(m, Locs(m), Graph(m))
+  }
+
+  function {:opaque} GetEntry(self: IndirectionTable, ref: BT.G.Reference) : (e : Option<Entry>)
+  requires Inv(self)
+  ensures e.None? ==> ref !in self.graph
+  ensures e.Some? ==> ref in self.graph
+  ensures e.Some? ==> self.graph[ref] == e.value.succs
+  ensures e.Some? && e.value.loc.Some? ==>
+      ref in self.locs && self.locs[ref] == e.value.loc.value
+  ensures ref in self.locs ==> e.Some? && e.value.loc.Some?
+  {
+    MutableMapModel.Get(self.t, ref)
+  }
+
+  predicate {:opaque} HasEmptyLoc(self: IndirectionTable, ref: BT.G.Reference)
+  requires Inv(self)
+  ensures HasEmptyLoc(self, ref) == (ref in self.graph && ref !in self.locs)
+  {
+    var entry := MutableMapModel.Get(self.t, ref);
+    entry.Some? && entry.value.loc.None?
+  }
+
+
+  function {:opaque} RemoveLocIfPresent(self: IndirectionTable, ref: BT.G.Reference) : (self' : IndirectionTable)
+  requires Inv(self)
+  ensures Inv(self')
+  ensures self'.locs == MapRemove1(self.locs, ref)
+  ensures self'.graph == self.graph
+  {
+    assume self.t.count as nat < 0x10000000000000000 / 8;
+    var oldEntry := MutableMapModel.Get(self.t, ref);
+    var t := (if oldEntry.Some? then
+      MutableMapModel.Insert(self.t, ref, Entry(None, oldEntry.value.succs))
+    else
+      self.t);
+    IndirectionTable(t, Locs(t), Graph(t))
+  }
+
+  function {:opaque} AddLocIfPresent(self: IndirectionTable, ref: BT.G.Reference, loc: BC.Location) : (IndirectionTable, bool)
+  requires Inv(self)
+  ensures var (self', added) := AddLocIfPresent(self, ref, loc);
+    && Inv(self')
+    && added == (ref in self.graph && ref !in self.locs)
+    && self'.graph == self.graph
+    && (added ==> self'.locs == self.locs[ref := loc])
+    && (!added ==> self'.locs == self.locs)
+  {
+    assume self.t.count as nat < 0x10000000000000000 / 8;
+    var oldEntry := MutableMapModel.Get(self.t, ref);
+    var added := oldEntry.Some? && oldEntry.value.loc.None?;
+    var t := (if added then
+      MutableMapModel.Insert(self.t, ref, Entry(Some(loc), oldEntry.value.succs))
+    else
+      self.t);
+    (IndirectionTable(t, Locs(t), Graph(t)), added)
+  }
+
+  function {:opaque} RemoveRef(self: IndirectionTable, ref: BT.G.Reference)
+    : (res : (IndirectionTable, Option<BC.Location>))
+  requires Inv(self)
+  ensures var (self', oldLoc) := res;
+    && Inv(self')
+    && self'.graph == MapRemove1(self.graph, ref)
+    && self'.locs == MapRemove1(self.locs, ref)
+    && (ref in self.locs ==> oldLoc == Some(self.locs[ref]))
+    && (ref !in self.locs ==> oldLoc == None)
+  {
+    var (t, oldEntry) := MutableMapModel.RemoveAndGet(self.t, ref);
+    var self' := IndirectionTable(t, Locs(t), Graph(t));
+    var oldLoc := if oldEntry.Some? then oldEntry.value.loc else None;
+    (self', oldLoc)
+  }
+
+  /*function updateRefcountsInc(garbageQueue: LruModel.LruQueue, refcounts: map<BT.G.Reference, uint64>, oldChildren: seq<BT.G.Reference, uint64>, newChildren: seq<BT.G.Reference>, idx: uint64)
+  requires 0 <= idx <= |newChildren|
+  {
+    if idx ==
+  }*/
+
+  function {:opaque} UpdateAndRemoveLoc(self: IndirectionTable, ref: BT.G.Reference, succs: seq<BT.G.Reference>) : (res : (IndirectionTable, Option<BC.Location>))
+  requires Inv(self)
+  ensures var (self', oldLoc) := res;
+    && Inv(self')
+    && self'.locs == MapRemove1(self.locs, ref)
+    && self'.graph == self.graph[ref := succs]
+    && (oldLoc.None? ==> ref !in self.locs)
+    && (oldLoc.Some? ==> ref in self.locs && self.locs[ref] == oldLoc.value)
+  {
+    assume self.t.count as nat < 0x10000000000000000 / 8;
+    var (t, oldEntry) := MutableMapModel.InsertAndGetOld(self.t, ref, Entry(None, succs));
+    var self' := IndirectionTable(t, Locs(t), Graph(t));
+    var oldLoc := if oldEntry.Some? && oldEntry.value.loc.Some? then oldEntry.value.loc else None;
+    (self', oldLoc)
+  }
+
+  function {:fuel ValInGrammar,3} valToHashMap(a: seq<V>) : (s : Option<HashMap>)
+  requires forall i | 0 <= i < |a| :: ValInGrammar(a[i], GTuple([GUint64, GUint64, GUint64, GUint64Array]))
+  ensures s.Some? ==> forall v | v in s.value.contents.Values :: v.loc.Some? && BC.ValidLocationForNode(v.loc.value)
+  {
+    if |a| == 0 then
+      Some(MutableMapModel.Constructor(1024))
+    else (
+      var res := valToHashMap(DropLast(a));
+      match res {
+        case Some(table) => (
+          var tuple := Last(a);
+          var ref := tuple.t[0].u;
+          var lba := tuple.t[1].u;
+          var len := tuple.t[2].u;
+          var succs := Some(tuple.t[3].ua);
+          match succs {
+            case None => None
+            case Some(succs) => (
+              var loc := LBAType.Location(lba, len);
+              if ref in table.contents || lba == 0 || !LBAType.ValidLocation(loc) then (
+                None
+              ) else (
+                assume table.count as nat < 0x10000000000000000 / 8;
+                Some(MutableMapModel.Insert(table, ref, Entry(Some(loc), succs)))
+              )
+            )
+          }
+        )
+        case None => None
+      }
+    )
+  }
+
+  function method IndirectionTableGrammar() : G
+  ensures ValidGrammar(IndirectionTableGrammar())
+  {
+    // (Reference, address, len, successor-list) triples
+    GArray(GTuple([GUint64, GUint64, GUint64, GUint64Array]))
+  }
+
+  function valToIndirectionTable(v: V) : (s : Option<IndirectionTable>)
+  requires ValInGrammar(v, IndirectionTableGrammar())
+  ensures s.Some? ==> Inv(s.value)
+  ensures s.Some? ==> BC.WFCompleteIndirectionTable(I(s.value))
+  {
+    var t := valToHashMap(v.a);
+    match t {
+      case Some(t) => (
+        var res := IndirectionTable(t, Locs(t), Graph(t));
+        if BT.G.Root() in res.graph && BC.GraphClosed(res.graph) then (
+          Some(res)
+        ) else (
+          None
+        )
+      )
+      case None => None
+    }
+  }
+
+  // To bitmap
+
+  predicate IsLocAllocIndirectionTable(indirectionTable: IndirectionTable, i: int)
+  {
+    || i == 0 // block 0 is always implicitly allocated
+    || !(
+      forall ref | ref in indirectionTable.locs ::
+        indirectionTable.locs[ref].addr as int != i * BlockSize() as int
+    )
+  }
+
+  predicate IsLocAllocBitmap(bm: Bitmap.BitmapModel, i: int)
+  {
+    && 0 <= i < Bitmap.Len(bm)
+    && Bitmap.IsSet(bm, i)
+  }
+
+  function InitLocBitmapIterate(indirectionTable: IndirectionTable,
+      it: MutableMapModel.Iterator<Entry>,
+      bm: Bitmap.BitmapModel)
+  : (res : (bool, Bitmap.BitmapModel))
+  requires Inv(indirectionTable)
+  requires MutableMapModel.WFIter(indirectionTable.t, it)
+  requires BC.WFCompleteIndirectionTable(I(indirectionTable))
+  requires Bitmap.Len(bm) == NumBlocks()
+  ensures Bitmap.Len(res.1) == NumBlocks()
+  decreases it.decreaser
+  {
+    if it.next.None? then (
+      (true, bm)
+    ) else (
+      var kv := it.next.value;
+      assert kv.0 in I(indirectionTable).locs;
+
+      var loc: uint64 := kv.1.loc.value.addr;
+      var locIndex: uint64 := loc / BlockSize() as uint64;
+      if locIndex < NumBlocks() as uint64 && !Bitmap.IsSet(bm, locIndex as int) then (
+        InitLocBitmapIterate(indirectionTable,
+            MutableMapModel.IterInc(indirectionTable.t, it),
+            Bitmap.BitSet(bm, locIndex as int))
+      ) else (
+        (false, bm)
+      )
+    )
+  }
+
+  function {:opaque} InitLocBitmap(indirectionTable: IndirectionTable) : (res : (bool, Bitmap.BitmapModel))
+  requires Inv(indirectionTable)
+  requires BC.WFCompleteIndirectionTable(I(indirectionTable))
+  ensures Bitmap.Len(res.1) == NumBlocks()
+  {
+    var bm := Bitmap.EmptyBitmap(NumBlocks());
+    var bm' := Bitmap.BitSet(bm, 0);
+    InitLocBitmapIterate(indirectionTable,
+        MutableMapModel.IterStart(indirectionTable.t),
+        bm')
+  }
+
+  predicate IsLocAllocIndirectionTablePartial(indirectionTable: IndirectionTable, i: int, s: set<uint64>)
+  {
+    || i == 0 // block 0 is always implicitly allocated
+    || !(
+      forall ref | ref in indirectionTable.locs && ref in s ::
+        indirectionTable.locs[ref].addr as int != i * BlockSize() as int
+    )
+  }
+
+  lemma InitLocBitmapIterateCorrect(indirectionTable: IndirectionTable,
+      it: MutableMapModel.Iterator<Entry>,
+      bm: Bitmap.BitmapModel)
+  requires Inv(indirectionTable)
+  requires InitLocBitmapIterate.requires(indirectionTable, it, bm);
+  requires (forall i: int ::
+        (IsLocAllocIndirectionTablePartial(indirectionTable, i, it.s)) <==> IsLocAllocBitmap(bm, i)
+      )
+  requires 
+    forall r1, r2 | r1 in I(indirectionTable).locs && r2 in I(indirectionTable).locs ::
+        r1 in it.s && r2 in it.s ==>
+        BC.LocationsForDifferentRefsDontOverlap(I(indirectionTable), r1, r2)
+  ensures var (succ, bm') := InitLocBitmapIterate(indirectionTable, it, bm);
+    (succ ==>
+      && (forall i: int ::
+        (IsLocAllocIndirectionTable(indirectionTable, i)
+        <==> IsLocAllocBitmap(bm', i)
+      ))
+      && BC.AllLocationsForDifferentRefsDontOverlap(I(indirectionTable))
+    )
+  decreases it.decreaser
+  {
+    Bitmap.reveal_BitSet();
+    Bitmap.reveal_IsSet();
+
+    var (succ, bm') := InitLocBitmapIterate(indirectionTable, it, bm);
+    if it.next.None? {
+      forall i: int | IsLocAllocIndirectionTable(indirectionTable, i)
+      ensures IsLocAllocBitmap(bm', i)
+      {
+      }
+
+      forall i: int
+      | IsLocAllocBitmap(bm', i)
+      ensures IsLocAllocIndirectionTable(indirectionTable, i)
+      {
+      }
+    } else {
+      if (succ) {
+        var kv := it.next.value;
+        assert kv.0 in indirectionTable.locs;
+        var loc: uint64 := kv.1.loc.value.addr;
+        var locIndex: uint64 := loc / BlockSize() as uint64;
+
+        //assert I(indirectionTable).locs[kv.0] == kv.1.0.value;
+        LBAType.reveal_ValidAddr();
+        assert BC.ValidLocationForNode(kv.1.loc.value);
+        assert locIndex as int * BlockSize() == loc as int;
+
+        //assert locIndex < NumBlocks() as uint64;
+        //assert !Bitmap.IsSet(bm, locIndex as int);
+
+        var bm0 := Bitmap.BitSet(bm, locIndex as int);
+        var it0 := MutableMapModel.IterInc(indirectionTable.t, it);
+
+        forall i: int
+        | IsLocAllocIndirectionTablePartial(indirectionTable, i, it0.s)
+        ensures IsLocAllocBitmap(bm0, i)
+        {
+          // This triggers all the right stuff:
+          if IsLocAllocIndirectionTablePartial(indirectionTable, i, it.s) { }
+          /*
+          if i != 0 {
+            var ref :| ref in indirectionTable.contents && indirectionTable.contents[ref].0.Some? && ref in it0.s && indirectionTable.contents[ref].0.value.addr as int == i * BlockSize() as int;
+            if (ref == kv.0) {
+              assert IsLocAllocBitmap(bm0, i);
+            } else {
+              assert IsLocAllocIndirectionTablePartial(indirectionTable, i, it.s);
+              assert IsLocAllocBitmap(bm0, i);
+            }
+          } else {
+            assert IsLocAllocIndirectionTablePartial(indirectionTable, i, it.s);
+          }
+          */
+        }
+
+        forall i: int
+        | IsLocAllocBitmap(bm0, i)
+        ensures IsLocAllocIndirectionTablePartial(indirectionTable, i, it0.s)
+        {
+          if IsLocAllocBitmap(bm, i) { }
+          if IsLocAllocIndirectionTablePartial(indirectionTable, i, it.s) { }
+
+          if i == locIndex as int {
+            var ref := kv.0;
+            assert indirectionTable.t.contents[ref].loc.Some?;
+            assert ref in it0.s;
+            assert indirectionTable.t.contents[ref] == kv.1;
+            assert indirectionTable.t.contents[ref].loc.value.addr as int == i * BlockSize() as int;
+
+            assert IsLocAllocIndirectionTablePartial(indirectionTable, i, it0.s);
+          } else {
+            assert IsLocAllocIndirectionTablePartial(indirectionTable, i, it0.s);
+          }
+        }
+
+        forall r1, r2 | r1 in I(indirectionTable).locs && r2 in I(indirectionTable).locs && r1 in it0.s && r2 in it0.s
+        ensures BC.LocationsForDifferentRefsDontOverlap(I(indirectionTable), r1, r2)
+        {
+          if r1 != r2 {
+            if r1 in it.s && r2 in it.s {
+              assert BC.LocationsForDifferentRefsDontOverlap(I(indirectionTable), r1, r2);
+            } else {
+              if I(indirectionTable).locs[r1].addr == I(indirectionTable).locs[r2].addr {
+                var j1 := LBAType.ValidAddrDivisor(I(indirectionTable).locs[r1].addr);
+                var j2 := LBAType.ValidAddrDivisor(I(indirectionTable).locs[r2].addr);
+                if r1 !in it.s {
+                  assert r2 in it.s;
+                  assert !Bitmap.IsSet(bm, j1);
+                  assert IsLocAllocBitmap(bm, j2);
+                  assert Bitmap.IsSet(bm, j2);
+                  assert false;
+                } else {
+                  assert r1 in it.s;
+                  assert !Bitmap.IsSet(bm, j2);
+                  assert IsLocAllocBitmap(bm, j1);
+                  assert Bitmap.IsSet(bm, j1);
+                  assert false;
+                }
+              } else {
+                assert BC.LocationsForDifferentRefsDontOverlap(I(indirectionTable), r1, r2);
+              }
+            }
+          }
+        }
+
+        InitLocBitmapIterateCorrect(indirectionTable, it0, bm0);
+        assert (succ, bm') == InitLocBitmapIterate(indirectionTable, it0, bm0);
+      }
+    }
+  }
+
+  lemma InitLocBitmapCorrect(indirectionTable: IndirectionTable)
+  requires Inv(indirectionTable)
+  requires BC.WFCompleteIndirectionTable(I(indirectionTable))
+  ensures var (succ, bm) := InitLocBitmap(indirectionTable);
+    (succ ==>
+      && (forall i: int :: IsLocAllocIndirectionTable(indirectionTable, i)
+        <==> IsLocAllocBitmap(bm, i)
+      )
+      && BC.AllLocationsForDifferentRefsDontOverlap(I(indirectionTable))
+    )
+  {
+    reveal_InitLocBitmap();
+    Bitmap.reveal_BitSet();
+    Bitmap.reveal_IsSet();
+
+    var it := MutableMapModel.IterStart(indirectionTable.t);
+
+    var bm := Bitmap.EmptyBitmap(NumBlocks());
+    var bm' := Bitmap.BitSet(bm, 0);
+
+    /*forall i: int | IsLocAllocIndirectionTablePartial(indirectionTable, i, it.s)
+    ensures IsLocAllocBitmap(bm', i)
+    {
+      assert i == 0;
+    }*/
+
+    forall i: int | IsLocAllocBitmap(bm', i)
+    ensures IsLocAllocIndirectionTablePartial(indirectionTable, i, it.s)
+    {
+      if i != 0 {
+        assert Bitmap.IsSet(bm', i)
+            == Bitmap.IsSet(bm, i)
+            == false;
+      }
+      assert i == 0;
+    }
+
+    InitLocBitmapIterateCorrect(indirectionTable, it, bm');
+  }
+
+  ///// Dealloc stuff
+
+  predicate deallocable(self: IndirectionTable, ref: BT.G.Reference)
+  {
+    && ref in I(self).graph
+    && ref != BT.G.Root()
+    && (forall r | r in I(self).graph :: ref !in I(self).graph[r])
+  }
+
+  function FindDeallocableIterate(self: IndirectionTable, ephemeralRefs: seq<BT.G.Reference>, i: uint64)
+  : (ref: Option<BT.G.Reference>)
+  requires 0 <= i as int <= |ephemeralRefs|
+  requires |ephemeralRefs| < 0x1_0000_0000_0000_0000;
+  decreases 0x1_0000_0000_0000_0000 - i as int
+  {
+    if i == |ephemeralRefs| as uint64 then (
+      None
+    ) else (
+      var ref := ephemeralRefs[i];
+      var isDeallocable := deallocable(self, ref);
+      if isDeallocable then (
+        Some(ref)
+      ) else (
+        FindDeallocableIterate(self, ephemeralRefs, i + 1)
+      )
+    )
+  }
+
+  function {:opaque} FindDeallocable(self: IndirectionTable)
+  : (ref: Option<BT.G.Reference>)
+  requires Inv(self)
+  {
+    // TODO once we have an lba freelist, rewrite this to avoid extracting a `map` from `s.ephemeralIndirectionTable`
+    var ephemeralRefs := setToSeq(self.t.contents.Keys);
+
+    assume |ephemeralRefs| < 0x1_0000_0000_0000_0000;
+
+    FindDeallocableIterate(self, ephemeralRefs, 0)
+  }
+
+  lemma FindDeallocableIterateCorrect(self: IndirectionTable, ephemeralRefs: seq<BT.G.Reference>, i: uint64)
+  requires Inv(self)
+  requires 0 <= i as int <= |ephemeralRefs|
+  requires |ephemeralRefs| < 0x1_0000_0000_0000_0000;
+  requires ephemeralRefs == setToSeq(self.t.contents.Keys)
+  requires forall k : nat | k < i as nat :: (
+        && ephemeralRefs[k] in I(self).graph
+        && !deallocable(self, ephemeralRefs[k]))
+  ensures var ref := FindDeallocableIterate(self, ephemeralRefs, i);
+      && (ref.Some? ==> ref.value in I(self).graph)
+      && (ref.Some? ==> deallocable(self, ref.value))
+      && (ref.None? ==> forall r | r in I(self).graph :: !deallocable(self, r))
+  decreases 0x1_0000_0000_0000_0000 - i as int
+  {
+    if i == |ephemeralRefs| as uint64 {
+      assert forall r | r in I(self).graph :: !deallocable(self, r);
+    } else {
+      var ref := ephemeralRefs[i];
+      var isDeallocable := deallocable(self, ref);
+      if isDeallocable {
+      } else {
+        FindDeallocableIterateCorrect(self, ephemeralRefs, i + 1);
+      }
+    }
+  }
+
+  lemma FindDeallocableCorrect(self: IndirectionTable)
+  requires Inv(self)
+  ensures var ref := FindDeallocable(self);
+      && (ref.Some? ==> ref.value in I(self).graph)
+      && (ref.Some? ==> deallocable(self, ref.value))
+      && (ref.None? ==> forall r | r in I(self).graph :: !deallocable(self, r))
+  {
+    reveal_FindDeallocable();
+    var ephemeralRefs := setToSeq(self.t.contents.Keys);
+    assume |ephemeralRefs| < 0x1_0000_0000_0000_0000;
+    FindDeallocableIterateCorrect(self, ephemeralRefs, 0);
+  }
+}
